formal/inference/heuristics/Store_Reuse.thy
@@ -154,7 +154,7 @@ lemmas remove_guard_add_update_preserves = remove_guard_add_update_preserves_lab
 
 definition is_generalisation_of :: "transition \<Rightarrow> transition \<Rightarrow> nat \<Rightarrow> nat \<Rightarrow> bool" where
   "is_generalisation_of t' t i r = (t' = remove_guard_add_update t i r \<and> 
-                                    i \<le> Arity t \<and> i > 0 \<and>
+                                    i < Arity t \<and>
                                     (\<exists>v. gexp.Eq (V (I i)) (L v) \<in> set (Guard t)) \<and>
                                     r \<notin> set (map fst (Updates t)))"
 
